Add evaluation based semantics for nnrc_imp #89

coq/NNRCimp/Lang/NNRCimpSem.v
@@ -35,213 +35,222 @@ Section NNRCimpSem.
   Require Import CommonRuntime.
   Require Import NNRCimp.
 
-    Context {fruntime:foreign_runtime}.
+  Context {fruntime:foreign_runtime}.
 
-    Context (h:brand_relation_t).
-    Context (σc:list (string*data)).
+  Context (h:brand_relation_t).
+  Context (σc:list (string*data)).
 
-    (* NB: normal variables and (unfrozen) mutable collection variables have *different namespaces*
+  (* NB: normal variables and (unfrozen) mutable collection variables have *different namespaces*
          Thus, when translating to another language without this distinction, care must be avoided to avoid 
           accidentally introducing shadowing.
-       *)
+   *)
 
-    Section Denotation.
+  Local Open Scope nnrc_imp.
+  Local Open Scope string.
 
-      Delimit Scope nnrc_imp with nnrc_imp_scope.
-      Reserved Notation  "[ σ ⊢〚 e 〛⇓ d ]". 
+  Section Denotation.
 
-      (* bindings that may or may not be initialized (defined) *)
-      Definition pd_bindings := list (string*option data).
+    Reserved Notation  "[ σ ⊢ e ⇓ d ]". 
 
-      Inductive nnrc_imp_expr_sem : pd_bindings -> nnrc_imp_expr -> data -> Prop :=
-      | sem_NNRCimpGetConstant : forall v σ d, 
-          edot σc v = Some d ->                 (**r   [Γc(v) = d] *)
-          [ σ ⊢〚 NNRCimpGetConstant v 〛⇓ d ]
-            
-      | sem_NNRCimpVar : forall v σ d,
-          lookup equiv_dec σ v = Some (Some d) ->              (**r   [Γ(v) = d] *)
-          [ σ ⊢〚 NNRCimpVar v 〛⇓ d ]
-            
-      | sem_NNRCimpConst : forall d₁ σ d₂,
-          normalize_data h d₁ = d₂ ->                     (**r   [norm(d₁) = d₂] *)
-          [ σ ⊢〚 NNRCimpConst d₁ 〛⇓ d₂ ]
-            
-      | sem_NNRCimpBinop : forall bop e₁ e₂ σ d₁ d₂ d,
-          [ σ ⊢〚 e₁ 〛⇓ d₁ ] ->
-          [ σ ⊢〚 e₂ 〛⇓ d₂ ] ->
-          [ σ ⊢〚 NNRCimpBinop bop e₁ e₂ 〛⇓ d ]
-            
-      | sem_NNRCimpUnop : forall uop e σ d₁ d,
-          [ σ ⊢〚 e 〛⇓ d₁ ] ->
-          nnrc_imp_expr_sem σ e d₁ ->             
-          unary_op_eval h uop d₁ = Some d ->     
-          [ σ ⊢〚 NNRCimpUnop uop e 〛⇓ d ]
+    Inductive nnrc_imp_expr_sem : pd_bindings -> nnrc_imp_expr -> data -> Prop :=
+    | sem_NNRCimpGetConstant : forall v σ d, 
+        edot σc v = Some d ->                 (**r   [Γc(v) = d] *)
+        [ σ ⊢ NNRCimpGetConstant v ⇓ d ]
+          
+    | sem_NNRCimpVar : forall v σ d,
+        lookup equiv_dec σ v = Some (Some d) ->              (**r   [Γ(v) = d] *)
+        [ σ ⊢ NNRCimpVar v ⇓ d ]
+          
+    | sem_NNRCimpConst : forall d₁ σ d₂,
+        normalize_data h d₁ = d₂ ->                     (**r   [norm(d₁) = d₂] *)
+        [ σ ⊢ NNRCimpConst d₁ ⇓ d₂ ]
+          
+    | sem_NNRCimpBinop : forall bop e₁ e₂ σ d₁ d₂ d,
+        [ σ ⊢ e₁ ⇓ d₁ ] ->
+        [ σ ⊢ e₂ ⇓ d₂ ] ->
+        [ σ ⊢ NNRCimpBinop bop e₁ e₂ ⇓ d ]
+          
+    | sem_NNRCimpUnop : forall uop e σ d₁ d,
+        [ σ ⊢ e ⇓ d₁ ] ->
+        nnrc_imp_expr_sem σ e d₁ ->             
+        unary_op_eval h uop d₁ = Some d ->     
+        [ σ ⊢ NNRCimpUnop uop e ⇓ d ]
 
-      | sem_NNRCimpGroupBy : forall g sl e σ d₁ d₂ ,
-          [ σ ⊢〚 e 〛⇓ (dcoll d₁) ] ->
-          group_by_nested_eval_table g sl d₁ = Some d₂ -> 
-          [ σ ⊢〚 NNRCimpGroupBy g sl e 〛⇓ (dcoll d₂) ]
-            
-      where
-      "[ σ ⊢〚 e 〛⇓ d ]" := (nnrc_imp_expr_sem σ e d) : nnrc_imp
-      .
+    | sem_NNRCimpGroupBy : forall g sl e σ d₁ d₂ ,
+        [ σ ⊢ e ⇓ (dcoll d₁) ] ->
+        group_by_nested_eval_table g sl d₁ = Some d₂ -> 
+        [ σ ⊢ NNRCimpGroupBy g sl e ⇓ (dcoll d₂) ]
+          
+    where
+    "[ σ ⊢ e ⇓ d ]" := (nnrc_imp_expr_sem σ e d) : nnrc_imp
+    .
+    
+    Reserved Notation  "[ σ₁ , ψ₁ ⊢ s₁ ⇓ σ₂ , ψ₂ ]". 
+    Reserved Notation "[ σ₁ , ψ₁ ⊢ s ⇓[ v <- dl ] σ₂ , ψ₂ ]".
 
-      Definition mut_coll_bindings := list (string*list data).
-      
-      Reserved Notation  "[ σ₁ , ψ₁ ⊢〚 s₁ 〛⇓ σ₂ , ψ₂ ]". 
-      Reserved Notation "[ σ₁ , ψ₁ ⊢〚 s 〛⇓[ v <- dl ] σ₂ , ψ₂ ]".
+    Inductive nnrc_imp_stmt_sem : pd_bindings -> mc_bindings -> nnrc_imp_stmt -> pd_bindings -> mc_bindings -> Prop :=
+    | sem_NNRCimpSeq s₁ s₂ σ₁ ψ₁ σ₂ ψ₂ σ₃ ψ₃  :
+        [ σ₁ , ψ₁ ⊢ s₁ ⇓ σ₂ , ψ₂ ] ->
+        [ σ₂ , ψ₂ ⊢ s₂ ⇓ σ₃ , ψ₃ ] ->
+        [ σ₁ , ψ₁ ⊢ NNRCimpSeq s₁ s₂ ⇓ σ₃ , ψ₃ ]
+          
+    | sem_NNRCimpLetMutInitialized v e s σ₁ ψ₁ σ₂ ψ₂ d dd :
+        [ σ₁ ⊢ e ⇓ d ] ->
+        [ (v,Some d)::σ₁, ψ₁ ⊢ s ⇓ (v,dd)::σ₂ , ψ₂ ] ->
+        [ σ₁ , ψ₁ ⊢ NNRCimpLetMut v (Some e) s ⇓ σ₂ , ψ₂ ]
+          
+    | sem_NNRCimpLetMutUninitialized v s σ₁ ψ₁ σ₂ ψ₂ dd :
+        [ (v,None)::σ₁, ψ₁ ⊢ s ⇓ (v,dd)::σ₂ , ψ₂ ] ->
+        [ σ₁ , ψ₁ ⊢ NNRCimpLetMut v None s ⇓ σ₂ , ψ₂ ]
+          
+    | sem_NNRCimpBuildCollFor v s₁ s₂ σ₁ ψ₁ σ₂ ψ₂ σ₃ ψ₃ d dd :
+        [ σ₁ , (v,nil)::ψ₁ ⊢ s₁ ⇓ σ₂ , (v,d)::ψ₂ ] ->
+        [ (v,Some (dcoll d))::σ₂ , ψ₂ ⊢ s₂ ⇓ (v,dd)::σ₃ , ψ₃ ] ->
+        [ σ₁ , ψ₁ ⊢ NNRCimpBuildCollFor v s₁ s₂ ⇓ σ₃ , ψ₃ ]
+          
+    | sem_NNRCimpPush v e σ ψ mc d :
+        lookup string_dec ψ v = Some mc ->
+        [ σ ⊢ e ⇓ d ] ->
+        [ σ , ψ ⊢ NNRCimpPush v e ⇓ σ , update_first string_dec ψ v (d::mc)]
+          
+    | sem_NNRCimpAssign v e σ ψ dold d :
+        lookup string_dec σ v = Some dold ->
+        [ σ ⊢ e ⇓ d ] ->
+        [ σ , ψ ⊢ NNRCimpAssign v e ⇓ update_first string_dec σ v (Some d), ψ]
+          
+    | sem_NNRCimpFor v e s σ₁ ψ₁ σ₂ ψ₂ dl :
+        [ σ₁ ⊢ e ⇓ (dcoll dl) ] ->
+        [ σ₁ , ψ₁ ⊢ s ⇓[v<-dl] σ₂, ψ₂] ->
+        [ σ₁ , ψ₁ ⊢ NNRCimpFor v e s ⇓ σ₂, ψ₂]
+          
+    | sem_NNRCimpIfTrue e s₁ s₂ σ₁ ψ₁ σ₂ ψ₂ :
+        [ σ₁ ⊢ e ⇓ (dbool true) ] ->
+        [ σ₁ , ψ₁ ⊢ s₁ ⇓ σ₂, ψ₂] ->
+        [ σ₁ , ψ₁ ⊢ NNRCimpIf e s₁ s₂ ⇓ σ₂, ψ₂]
+          
+    | sem_NNRCimpIfFalse e s₁ s₂ σ₁ ψ₁ σ₂ ψ₂ :
+        [ σ₁ ⊢ e ⇓ (dbool false) ] ->
+        [ σ₁ , ψ₁ ⊢ s₂ ⇓ σ₂, ψ₂] ->
+        [ σ₁ , ψ₁ ⊢ NNRCimpIf e s₁ s₂ ⇓ σ₂, ψ₂]
+          
+    | sem_NNRCimpEitherLeft e x₁ s₁ x₂ s₂ σ₁ ψ₁ σ₂ ψ₂ d dd :
+        [ σ₁ ⊢ e ⇓ (dleft d) ] ->
+        [ (x₁,Some d)::σ₁ , ψ₁ ⊢ s₁ ⇓ (x₁,dd)::σ₂, ψ₂] ->
+        [ σ₁ , ψ₁ ⊢ NNRCimpEither e x₁ s₁ x₂ s₂ ⇓ σ₂, ψ₂]
+          
+    | sem_NNRCimpEitherRight e x₁ s₁ x₂ s₂ σ₁ ψ₁ σ₂ ψ₂ d dd :
+        [ σ₁ ⊢ e ⇓ (dleft d) ] ->
+        [ (x₂,Some d)::σ₁ , ψ₁ ⊢ s₂ ⇓ (x₂,dd)::σ₂, ψ₂] ->
+        [ σ₁ , ψ₁ ⊢ NNRCimpEither e x₁ s₁ x₂ s₂ ⇓ σ₂, ψ₂]
+          
+    with nnrc_imp_stmt_sem_iter: var -> list data -> pd_bindings -> mc_bindings -> nnrc_imp_stmt -> pd_bindings -> mc_bindings -> Prop :=
+         | sem_NNRCimpIter_nil v s σ ψ :
+             [ σ , ψ ⊢ s ⇓[v<-nil] σ, ψ]
+         | sem_NNRCimpIter_cons v s σ₁ ψ₁ σ₂ ψ₂ σ₃ ψ₃ d dl dd:
+             [ (v,Some d)::σ₁, ψ₁ ⊢ s ⇓ (v,dd)::σ₂, ψ₂] ->
+             [ σ₂ , ψ₂ ⊢ s ⇓[v<-dl] σ₃, ψ₃] ->
+             [ σ₁ , ψ₁ ⊢ s ⇓[v<-d::dl] σ₃, ψ₃]
+    where
+    "[ σ₁ , ψ₁ ⊢ s ⇓ σ₂ , ψ₂ ]" := (nnrc_imp_stmt_sem σ₁ ψ₁ s σ₂ ψ₂ ) : nnrc_imp
+                                                                          and "[ σ₁ , ψ₁ ⊢ s ⇓[ v <- dl ] σ₂ , ψ₂ ]" := (nnrc_imp_stmt_sem_iter v dl σ₁ ψ₁ s σ₂ ψ₂ ) : nnrc_imp.
 
-      Inductive nnrc_imp_stmt_sem : pd_bindings -> mut_coll_bindings -> nnrc_imp_stmt -> pd_bindings -> mut_coll_bindings -> Prop :=
-      | sem_NNRCimpSeq s₁ s₂ σ₁ ψ₁ σ₂ ψ₂ σ₃ ψ₃  :
-          [ σ₁ , ψ₁ ⊢〚 s₁ 〛⇓ σ₂ , ψ₂ ] ->
-          [ σ₂ , ψ₂ ⊢〚 s₂ 〛⇓ σ₃ , ψ₃ ] ->
-          [ σ₁ , ψ₁ ⊢〚 NNRCimpSeq s₁ s₂ 〛⇓ σ₃ , ψ₃ ]
-            
-      | sem_NNRCimpLetMutInitialized v e s σ₁ ψ₁ σ₂ ψ₂ d dd :
-          [ σ₁ ⊢〚 e 〛⇓ d ] ->
-          [ (v,Some d)::σ₁, ψ₁ ⊢〚 s 〛⇓ (v,dd)::σ₂ , ψ₂ ] ->
-          [ σ₁ , ψ₁ ⊢〚 NNRCimpLetMut v (Some e) s 〛⇓ σ₂ , ψ₂ ]
-            
-      | sem_NNRCimpLetMutUninitialized v s σ₁ ψ₁ σ₂ ψ₂ dd :
-          [ (v,None)::σ₁, ψ₁ ⊢〚 s 〛⇓ (v,dd)::σ₂ , ψ₂ ] ->
-          [ σ₁ , ψ₁ ⊢〚 NNRCimpLetMut v None s 〛⇓ σ₂ , ψ₂ ]
-            
-      | sem_NNRCimpBuildCollFor v s₁ s₂ σ₁ ψ₁ σ₂ ψ₂ σ₃ ψ₃ d dd :
-          [ σ₁ , (v,nil)::ψ₁ ⊢〚 s₁ 〛⇓ σ₂ , (v,d)::ψ₂ ] ->
-          [ (v,Some (dcoll d))::σ₂ , ψ₂ ⊢〚 s₂ 〛⇓ (v,dd)::σ₃ , ψ₃ ] ->
-          [ σ₁ , ψ₁ ⊢〚 NNRCimpBuildCollFor v s₁ s₂ 〛⇓ σ₃ , ψ₃ ]
-            
-      | sem_NNRCimpPush v e σ ψ mc d :
-          lookup string_dec ψ v = Some mc ->
-          [ σ ⊢〚 e 〛⇓ d ] ->
-          [ σ , ψ ⊢〚 NNRCimpPush v e 〛⇓ σ , update_first string_dec ψ v (d::mc)]
-            
-      | sem_NNRCimpAssign v e σ ψ dold d :
-          lookup string_dec σ v = Some dold ->
-          [ σ ⊢〚 e 〛⇓ d ] ->
-          [ σ , ψ ⊢〚 NNRCimpAssign v e 〛⇓ update_first string_dec σ v (Some d), ψ]
-            
-      | sem_NNRCimpFor v e s σ₁ ψ₁ σ₂ ψ₂ dl :
-          [ σ₁ ⊢〚 e 〛⇓ (dcoll dl) ] ->
-          [ σ₁ , ψ₁ ⊢〚 s 〛⇓[v<-dl] σ₂, ψ₂] ->
-          [ σ₁ , ψ₁ ⊢〚 NNRCimpFor v e s 〛⇓ σ₂, ψ₂]
-            
-      | sem_NNRCimpIfTrue e s₁ s₂ σ₁ ψ₁ σ₂ ψ₂ :
-          [ σ₁ ⊢〚 e 〛⇓ (dbool true) ] ->
-          [ σ₁ , ψ₁ ⊢〚 s₁ 〛⇓ σ₂, ψ₂] ->
-          [ σ₁ , ψ₁ ⊢〚 NNRCimpIf e s₁ s₂ 〛⇓ σ₂, ψ₂]
-            
-      | sem_NNRCimpIfFalse e s₁ s₂ σ₁ ψ₁ σ₂ ψ₂ :
-          [ σ₁ ⊢〚 e 〛⇓ (dbool false) ] ->
-          [ σ₁ , ψ₁ ⊢〚 s₂ 〛⇓ σ₂, ψ₂] ->
-          [ σ₁ , ψ₁ ⊢〚 NNRCimpIf e s₁ s₂ 〛⇓ σ₂, ψ₂]
-            
-      | sem_NNRCimpEitherLeft e x₁ s₁ x₂ s₂ σ₁ ψ₁ σ₂ ψ₂ d dd :
-          [ σ₁ ⊢〚 e 〛⇓ (dleft d) ] ->
-          [ (x₁,Some d)::σ₁ , ψ₁ ⊢〚 s₁ 〛⇓ (x₁,dd)::σ₂, ψ₂] ->
-          [ σ₁ , ψ₁ ⊢〚 NNRCimpEither e x₁ s₁ x₂ s₂ 〛⇓ σ₂, ψ₂]
-            
-      | sem_NNRCimpEitherRight e x₁ s₁ x₂ s₂ σ₁ ψ₁ σ₂ ψ₂ d dd :
-          [ σ₁ ⊢〚 e 〛⇓ (dleft d) ] ->
-          [ (x₂,Some d)::σ₁ , ψ₁ ⊢〚 s₂ 〛⇓ (x₂,dd)::σ₂, ψ₂] ->
-          [ σ₁ , ψ₁ ⊢〚 NNRCimpEither e x₁ s₁ x₂ s₂ 〛⇓ σ₂, ψ₂]
-      
-      with nnrc_imp_stmt_sem_iter: var -> list data -> pd_bindings -> mut_coll_bindings -> nnrc_imp_stmt -> pd_bindings -> mut_coll_bindings -> Prop :=
-           | sem_NNRCimpIter_nil v s σ ψ :
-               [ σ , ψ ⊢〚 s 〛⇓[v<-nil] σ, ψ]
-           | sem_NNRCimpIter_cons v s σ₁ ψ₁ σ₂ ψ₂ σ₃ ψ₃ d dl dd:
-               [ (v,Some d)::σ₁, ψ₁ ⊢〚 s 〛⇓ (v,dd)::σ₂, ψ₂] ->
-               [ σ₂ , ψ₂ ⊢〚 s 〛⇓[v<-dl] σ₃, ψ₃] ->
-               [ σ₁ , ψ₁ ⊢〚 s 〛⇓[v<-d::dl] σ₃, ψ₃]
-      where
-      "[ σ₁ , ψ₁ ⊢〚 s 〛⇓ σ₂ , ψ₂ ]" := (nnrc_imp_stmt_sem σ₁ ψ₁ s σ₂ ψ₂ ) : nnrc_imp
-      and "[ σ₁ , ψ₁ ⊢〚 s 〛⇓[ v <- dl ] σ₂ , ψ₂ ]" := (nnrc_imp_stmt_sem_iter v dl σ₁ ψ₁ s σ₂ ψ₂ ) : nnrc_imp.
+    Notation "[ σ₁ , ψ₁ ⊢ s ⇓ σ₂ , ψ₂ ]" := (nnrc_imp_stmt_sem σ₁ ψ₁ s σ₂ ψ₂ ) : nnrc_imp.
+    Notation "[ σ₁ , ψ₁ ⊢ s ⇓[ v <- dl ] σ₂ , ψ₂ ]" := (nnrc_imp_stmt_sem_iter v dl σ₁ ψ₁ s σ₂ ψ₂ ) : nnrc_imp.
 
-      Notation "[ σ₁ , ψ₁ ⊢〚 s 〛⇓ σ₂ , ψ₂ ]" := (nnrc_imp_stmt_sem σ₁ ψ₁ s σ₂ ψ₂ ) : nnrc_imp.
-      Notation "[ σ₁ , ψ₁ ⊢〚 s 〛⇓[ v <- dl ] σ₂ , ψ₂ ]" := (nnrc_imp_stmt_sem_iter v dl σ₁ ψ₁ s σ₂ ψ₂ ) : nnrc_imp.
+    Reserved Notation "[  s ⇓[ ret ] d  ]".
 
-      Local Open Scope nnrc_imp.
-
-      Reserved Notation "[ 〚 s 〛⇓[ ret ] d  ]".
-
-      Inductive nnrc_imp_stmt_sem_top_ret (ret:string) : nnrc_imp -> data -> Prop :=
+    Inductive nnrc_imp_stmt_sem_top_ret (ret:string) :
+      nnrc_imp -> data -> Prop
+      :=
       | sem_NNRCimpTopRet s d :
-          [ (ret,None)::nil , nil ⊢〚 s 〛⇓ (ret, Some d)::nil, nil ] ->
-          [  〚 s 〛⇓[ ret ] d  ]
-      where
-      "[  〚 s 〛⇓[ ret ] d  ]" := (nnrc_imp_stmt_sem_top_ret ret s d ) : nnrc_imp.
+          [ (ret,None)::nil , nil ⊢ s ⇓ (ret, Some d)::nil, nil ] ->
+          [   s ⇓[ ret ] d  ]
+    where
+    "[   s ⇓[ ret ] d  ]" := (nnrc_imp_stmt_sem_top_ret ret s d ) : nnrc_imp.
 
-      Notation "[  〚  s 〛⇓[ ret ] d  ]" := (nnrc_imp_stmt_sem_top_ret ret s d ) : nnrc_imp.
+    Notation "[    s ⇓[ ret ] d  ]" := (nnrc_imp_stmt_sem_top_ret ret s d ) : nnrc_imp.
 
-      Local Open Scope string.
+    Local Open Scope string.
+    
+  End Denotation.
 
-      Lemma nnrc_imp_stmt_env_stack s σ₁ ψ₁ σ₂ ψ₂ :
-        [ σ₁ , ψ₁ ⊢〚 s 〛⇓ σ₂ , ψ₂ ] -> domain σ₁ = domain σ₂.
-      Proof.
-        revert σ₁ ψ₁ σ₂ ψ₂.
-        nnrc_imp_stmt_cases (induction s) Case; intros σ₁ ψ₁ σ₂ ψ₂ sem; invcs sem.
-        - Case "NNRCimpSeq".
-          transitivity (domain σ₂0); eauto.
-        - Case "NNRCimpLetMut".
-          specialize (IHs _ _ _ _ H7).
-          simpl in IHs; invcs IHs.
-          trivial.
-        - Case "NNRCimpLetMut".
-          specialize (IHs _ _ _ _ H6).
-          simpl in IHs; invcs IHs.
-          trivial.
-        - Case "NNRCimpBuildCollFor".
-          specialize (IHs1 _ _ _ _ H6).
-          specialize (IHs2 _ _ _ _ H7).
-          simpl in IHs2; invcs IHs2.
-          congruence.
-        - Case "NNRCimpPush".
-          trivial.
-        - Case "NNRCimpAssign".
-          rewrite domain_update_first; trivial.
-        - Case  "NNRCimpFor".
-          clear H6.
-          revert σ₁ ψ₁ σ₂ ψ₂ H7.
-          induction dl; intros σ₁ ψ₁ σ₂ ψ₂ sem; invcs sem; trivial.
-          specialize (IHdl _ _ _ _ H8).
-          specialize (IHs _ _ _ _ H2).
-          simpl in IHs; invcs IHs.
-          congruence.
-        - Case "NNRCimpIf".
-          eauto.
-        - Case "NNRCimpIf".
-          eauto.
-        - Case "NNRCimpEither".
-          specialize (IHs1 _ _ _ _ H9).
-          simpl in IHs1; invcs IHs1; trivial.
-        - Case "NNRCimpEither".
-          specialize (IHs2 _ _ _ _ H9).
-          simpl in IHs2; invcs IHs2; trivial.
-      Qed.
+  Notation "[ σ ⊢ e ⇓ d ]" := (nnrc_imp_expr_sem σ e d) : nnrc_imp.
+  Notation "[ σ₁ , ψ₁ ⊢ s ⇓ σ₂ , ψ₂ ]" := (nnrc_imp_stmt_sem σ₁ ψ₁ s σ₂ ψ₂ ) : nnrc_imp.
+  Notation "[ σ₁ , ψ₁ ⊢ s ⇓[ v <- dl ] σ₂ , ψ₂ ]" := (nnrc_imp_stmt_sem_iter v dl σ₁ ψ₁ s σ₂ ψ₂ ) : nnrc_imp.
 
-      Lemma nnrc_imp_stmt_mut_coll_stack s σ₁ ψ₁ σ₂ ψ₂ :
-        [ σ₁ , ψ₁ ⊢〚 s 〛⇓ σ₂ , ψ₂ ] -> domain ψ₁ = domain ψ₂.
-      Proof.
-        revert σ₁ ψ₁ σ₂ ψ₂.
-        nnrc_imp_stmt_cases (induction s) Case; intros σ₁ ψ₁ σ₂ ψ₂ sem; invcs sem; eauto.
-        - Case "NNRCimpSeq".
-          transitivity (domain ψ₂0); eauto.
-        - Case "NNRCimpBuildCollFor".
-          specialize (IHs1 _ _ _ _ H6).
-          specialize (IHs2 _ _ _ _ H7).
-          simpl in IHs1; invcs IHs1.
-          congruence.
-        - Case "NNRCimpPush".
-          rewrite domain_update_first; trivial.
-        - Case  "NNRCimpFor".
-          clear H6.
-          revert σ₁ ψ₁ σ₂ ψ₂ H7.
-          induction dl; intros σ₁ ψ₁ σ₂ ψ₂ sem; invcs sem; trivial.
-          specialize (IHdl _ _ _ _ H8).
-          specialize (IHs _ _ _ _ H2).
-          congruence.
-      Qed.
-                 
-    End Denotation.
 
+  Section props.
+    
+    Lemma nnrc_imp_stmt_sem_env_stack s σ₁ ψ₁ σ₂ ψ₂ :
+      [ σ₁ , ψ₁ ⊢ s ⇓ σ₂ , ψ₂ ] -> domain σ₁ = domain σ₂.
+    Proof.
+      revert σ₁ ψ₁ σ₂ ψ₂.
+      nnrc_imp_stmt_cases (induction s) Case; intros σ₁ ψ₁ σ₂ ψ₂ sem; invcs sem.
+      - Case "NNRCimpSeq".
+        transitivity (domain σ₂0); eauto.
+      - Case "NNRCimpLetMut".
+        specialize (IHs _ _ _ _ H7).
+        simpl in IHs; invcs IHs.
+        trivial.
+      - Case "NNRCimpLetMut".
+        specialize (IHs _ _ _ _ H6).
+        simpl in IHs; invcs IHs.
+        trivial.
+      - Case "NNRCimpBuildCollFor".
+        specialize (IHs1 _ _ _ _ H6).
+        specialize (IHs2 _ _ _ _ H7).
+        simpl in IHs2; invcs IHs2.
+        congruence.
+      - Case "NNRCimpPush".
+        trivial.
+      - Case "NNRCimpAssign".
+        rewrite domain_update_first; trivial.
+      - Case  "NNRCimpFor".
+        clear H6.
+        revert σ₁ ψ₁ σ₂ ψ₂ H7.
+        induction dl; intros σ₁ ψ₁ σ₂ ψ₂ sem; invcs sem; trivial.
+        specialize (IHdl _ _ _ _ H8).
+        specialize (IHs _ _ _ _ H2).
+        simpl in IHs; invcs IHs.
+        congruence.
+      - Case "NNRCimpIf".
+        eauto.
+      - Case "NNRCimpIf".
+        eauto.
+      - Case "NNRCimpEither".
+        specialize (IHs1 _ _ _ _ H9).
+        simpl in IHs1; invcs IHs1; trivial.
+      - Case "NNRCimpEither".
+        specialize (IHs2 _ _ _ _ H9).
+        simpl in IHs2; invcs IHs2; trivial.
+    Qed.
+
+    Lemma nnrc_imp_stmt_sem_mcenv_stack s σ₁ ψ₁ σ₂ ψ₂ :
+      [ σ₁ , ψ₁ ⊢ s ⇓ σ₂ , ψ₂ ] -> domain ψ₁ = domain ψ₂.
+    Proof.
+      revert σ₁ ψ₁ σ₂ ψ₂.
+      nnrc_imp_stmt_cases (induction s) Case; intros σ₁ ψ₁ σ₂ ψ₂ sem; invcs sem; eauto.
+      - Case "NNRCimpSeq".
+        transitivity (domain ψ₂0); eauto.
+      - Case "NNRCimpBuildCollFor".
+        specialize (IHs1 _ _ _ _ H6).
+        specialize (IHs2 _ _ _ _ H7).
+        simpl in IHs1; invcs IHs1.
+        congruence.
+      - Case "NNRCimpPush".
+        rewrite domain_update_first; trivial.
+      - Case  "NNRCimpFor".
+        clear H6.
+        revert σ₁ ψ₁ σ₂ ψ₂ H7.
+        induction dl; intros σ₁ ψ₁ σ₂ ψ₂ sem; invcs sem; trivial.
+        specialize (IHdl _ _ _ _ H8).
+        specialize (IHs _ _ _ _ H2).
+        congruence.
+    Qed.
+
+  End props.
+  
 End NNRCimpSem.
+Notation "[ h , σc ; σ ⊢ e ⇓ d ]" := (nnrc_imp_expr_sem h σc σ e d) : nnrc_imp.
+Notation "[ h , σc ; σ₁ , ψ₁ ⊢ s ⇓ σ₂ , ψ₂ ]" := (nnrc_imp_stmt_sem h σc σ₁ ψ₁ s σ₂ ψ₂ ) : nnrc_imp.
+Notation "[ h , σc ; σ₁ , ψ₁ ⊢ s ⇓[ v <- dl ] σ₂ , ψ₂ ]" := (nnrc_imp_stmt_sem_iter h σc v dl σ₁ ψ₁ s σ₂ ψ₂ ) : nnrc_imp.
