coq/NNRCimp/Lang/NNRCImpEval.v
@@ -1,0 +1,297 @@
+(*
+ * Copyright 2015-2016 IBM Corporation
+ *
+ * Licensed under the Apache License, Version 2.0 (the "License");
+ * you may not use this file except in compliance with the License.
+ * You may obtain a copy of the License at
+ *
+ * http://www.apache.org/licenses/LICENSE-2.0
+ *
+ * Unless required by applicable law or agreed to in writing, software
+ * distributed under the License is distributed on an "AS IS" BASIS,
+ * WITHOUT WARRANTIES OR CONDITIONS OF ANY KIND, either express or implied.
+ * See the License for the specific language governing permissions and
+ * limitations under the License.
+ *)
+
+(** NNRCimp is a variant of the named nested relational calculus
+     (NNRC) that is meant to be more imperative in feel.  It is used
+     as an intermediate language between NNRC and more imperative /
+     statement oriented backends *)
+
+Section NNRCimpEval.
+  Require Import String.
+  Require Import List.
+  Require Import Arith.
+  Require Import EquivDec.
+  Require Import Morphisms.
+  Require Import Arith.
+  Require Import Max.
+  Require Import Bool.
+  Require Import Peano_dec.
+  Require Import EquivDec.
+  Require Import Decidable.
+  Require Import Utils.
+  Require Import CommonRuntime.
+  Require Import NNRCimp.
+
+  Context {fruntime:foreign_runtime}.
+
+  Context (h:brand_relation_t).
+  Context (σc:list (string*data)).
+
+  Local Open Scope nnrc_imp.
+  Local Open Scope string.
+
+  (** ** Evaluation Semantics *)
+  Section Evaluation.
+
+    (** Evaluation takes a NNRCimp expression and an environment. It
+          returns an optional value. When [None] is returned, it
+          denotes an error. An error is always propagated. *)
+
+
+    Reserved Notation  "[ σ ⊢〚 e 〛 ]". 
+
+    Fixpoint nnrc_imp_expr_eval
+             (σ:pd_bindings) (e:nnrc_imp_expr)
+      : option data
+      := match e with
+         | NNRCimpGetConstant v =>
+           edot σc v
+                
+         | NNRCimpVar v =>
+           olift id (lookup equiv_dec σ v)
+                 
+         | NNRCimpConst d =>
+           Some (normalize_data h d)
+                
+         | NNRCimpBinop bop e₁ e₂ =>
+           olift2 (fun d₁ d₂ => binary_op_eval h bop d₁ d₂)
+                  ([ σ ⊢〚 e₁ 〛 ])
+                  ([ σ ⊢〚 e₂ 〛 ])
+                  
+         | NNRCimpUnop uop e =>
+           olift (fun d => unary_op_eval h uop d)
+                 ([ σ ⊢〚 e 〛 ])
+                 
+         | NNRCimpGroupBy g sl e =>
+           match [ σ ⊢〚 e 〛 ] with
+           | Some (dcoll dl) => lift dcoll (group_by_nested_eval_table g sl dl)
+           | _ => None
+           end
+         end
+    where "[ σ ⊢〚 e 〛 ]" := (nnrc_imp_expr_eval σ e) : nnrc_imp. 
+
+    Reserved Notation  "[ σ , ψ ⊢〚 s 〛 ]". 
+
+    Fixpoint nnrc_imp_stmt_eval
+             (σ:pd_bindings) (ψ:mc_bindings)
+             (s:nnrc_imp_stmt) : option (pd_bindings*mc_bindings)
+      := match s with
+         | NNRCimpSeq s₁ s₂ =>
+           match [ σ , ψ ⊢〚 s₁ 〛] with
+           | Some (σ₁, ψ₁) => [ σ₁ , ψ₁ ⊢〚 s₂ 〛 ]
+           | None => None
+           end
+             
+         | NNRCimpLetMut v (Some e) s₀ =>
+           match [ σ  ⊢〚 e 〛] with
+           | Some d =>
+             match [ ((v,Some d)::σ) , ψ ⊢〚 s₀ 〛 ]  with
+             | Some (_::σ₁, ψ₁) => Some (σ₁, ψ₁)
+             | _ => None
+             end
+           | None => None
+           end
+             
+         | NNRCimpLetMut v None s₀ =>
+           match [ ((v,None)::σ), ψ ⊢〚 s₀ 〛 ] with
+           | Some (_::σ₁, ψ₁) => Some (σ₁, ψ₁)
+           | _ => None
+           end
+             
+         | NNRCimpBuildCollFor v s₁ s₂ =>
+           match [ σ, ((v,nil)::ψ) ⊢〚s₁〛]  with
+           | Some (σ₁, ((_,dl)::ψ₁)) =>
+             match [ ((v,Some (dcoll dl))::σ₁), ψ₁ ⊢〚s₂〛]  with
+             | Some ((_::σ₂),ψ₂) => Some (σ₂,ψ₂)
+             | _ => None
+             end
+           | _ => None
+           end
+             
+         | NNRCimpPush v e =>
+           match [ σ  ⊢〚 e 〛] , lookup string_dec ψ v with
+           | Some d, Some dl => Some (σ, update_first string_dec ψ v (d::dl))
+           | _, _ => None
+           end
+             
+         | NNRCimpAssign v e =>
+           match [ σ  ⊢〚 e 〛] , lookup string_dec σ v with
+           | Some d, Some _ => Some (update_first string_dec σ v (Some d), ψ)
+           | _, _ => None
+           end
+             
+         | NNRCimpFor v e s₀ =>
+           match [ σ  ⊢〚 e 〛]  with
+           | Some (dcoll c1) =>
+             let fix for_fun (dl:list data) σ₁ ψ₁ :=
+                 match dl with
+                 | nil => Some (σ₁, ψ₁)
+                 | d::dl' => 
+                   match [ ((v,Some d)::σ₁), ψ₁ ⊢〚 s₀ 〛 ] with
+                   | Some (_::σ₂, ψ₂) => for_fun dl' σ₂ ψ₂
+                   | _ => None
+                   end
+                 end in
+             for_fun c1 σ ψ
+           | _ => None
+           end
+             
+         | NNRCimpIf e s₁ s₂ =>
+           match [ σ  ⊢〚 e 〛]  with
+           | Some (dbool true) => [ σ, ψ ⊢〚 s₁ 〛]
+           | Some (dbool false) => [ σ, ψ ⊢〚 s₂ 〛] 
+           | _ => None
+           end
+             
+         | NNRCimpEither e x₁ s₁ x₂ s₂ =>
+           match [ σ  ⊢〚 e 〛] with
+           | Some (dleft d) =>
+             match [ ((x₁,Some d)::σ), ψ ⊢〚 s₁ 〛] with
+             | Some (_::σ₂, ψ₂) => Some (σ₂, ψ₂)
+             | _ => None
+             end
+           | Some (dright d) =>
+             match  [ ((x₂,Some d)::σ), ψ ⊢〚 s₂ 〛]with
+             | Some (_::σ₂, ψ₂) => Some (σ₂, ψ₂)
+             | _ => None
+             end
+           | _ => None
+           end
+         end
+    where "[ σ , ψ ⊢〚 s 〛 ]" := (nnrc_imp_stmt_eval σ ψ s) : nnrc_imp. 
+
+  End Evaluation.
+
+  Notation "[ σ ⊢〚 e 〛 ]" := (nnrc_imp_expr_eval σ e) : nnrc_imp. 
+  Notation "[ σ , ψ ⊢〚 s 〛 ]" := (nnrc_imp_stmt_eval σ ψ s) : nnrc_imp.
+
+  Section props.
+
+    Ltac destr H :=
+      let eqq := fresh "eqq" in
+      first [(match_case_in H;
+              [intros [??] eqq | intros eqq]; rewrite eqq in H; try discriminate)
+            | (match_case_in H;
+               [intros ? eqq | intros eqq]; rewrite eqq in H; try discriminate)
+            | (match_case_in H;
+               [intros eqq | intros ? ? eqq]; try rewrite eqq in H; try discriminate)
+            | (match_case_in H;
+               [intros eqq | intros ? eqq]; try rewrite eqq in H; try discriminate)
+            ]; subst.
+      
+    Lemma nnrc_imp_stmt_eval_env_stack s σ₁ ψ₁ σ₂ ψ₂ :
+      [ σ₁ , ψ₁ ⊢〚 s〛] = Some (σ₂ , ψ₂ ) -> domain σ₁ = domain σ₂.
+    Proof.
+      revert σ₁ ψ₁ σ₂ ψ₂.
+      nnrc_imp_stmt_cases (induction s) Case; intros σ₁ ψ₁ σ₂ ψ₂ sem; simpl in sem; repeat destr sem.
+      - Case "NNRCimpSeq".
+        transitivity (domain p); eauto.
+      - Case "NNRCimpLetMut".
+        invcs sem.
+        specialize (IHs _ _ _ _ eqq0).
+        simpl in IHs; invcs IHs; trivial.
+      - Case "NNRCimpLetMut".
+        invcs sem.
+        specialize (IHs _ _ _ _ eqq).
+        simpl in IHs; invcs IHs; trivial.
+      - Case "NNRCimpBuildCollFor".
+        destruct p0; repeat destr sem.
+        specialize (IHs1 _ _ _ _ eqq).
+        specialize (IHs2 _ _ _ _ eqq0).
+        simpl in IHs2; invcs IHs2.
+        congruence.
+      - Case "NNRCimpPush".
+        invcs sem; trivial.
+      - Case "NNRCimpAssign".
+        invcs sem.
+        rewrite domain_update_first; trivial.
+      - Case  "NNRCimpFor".
+        destruct d; try discriminate.
+        clear eqq.
+        revert σ₁ ψ₁ σ₂ ψ₂ sem.
+        induction l; intros σ₁ ψ₁ σ₂ ψ₂ sem; invcs sem; trivial.
+        repeat destr H0.
+        specialize (IHl _ _ _ _ H0).
+        specialize (IHs _ _ _ _ eqq).
+        simpl in IHs; invcs IHs.
+        congruence.
+      - Case "NNRCimpIf".
+        destruct d; try discriminate.
+        destruct b; eauto.
+      - Case "NNRCimpEither".
+        destruct d; try discriminate;
+          repeat destr sem; invcs sem.
+        + specialize (IHs1 _ _ _ _ eqq0);
+            simpl in IHs1; invcs IHs1; trivial.
+        + specialize (IHs2 _ _ _ _ eqq0);
+            simpl in IHs2; invcs IHs2; trivial.
+    Qed.
+
+    Lemma nnrc_imp_stmt_eval_mcenv_stack s σ₁ ψ₁ σ₂ ψ₂ :
+      [ σ₁ , ψ₁ ⊢〚 s〛] = Some (σ₂ , ψ₂ ) -> domain ψ₁ = domain ψ₂.
+    Proof.
+      revert σ₁ ψ₁ σ₂ ψ₂.
+      nnrc_imp_stmt_cases (induction s) Case; intros σ₁ ψ₁ σ₂ ψ₂ sem; simpl in sem; repeat destr sem.
+      - Case "NNRCimpSeq".
+        transitivity (domain m); eauto.
+      - Case "NNRCimpLetMut".
+        invcs sem.
+        specialize (IHs _ _ _ _ eqq0).
+        simpl in IHs; invcs IHs; trivial.
+      - Case "NNRCimpLetMut".
+        invcs sem.
+        specialize (IHs _ _ _ _ eqq).
+        simpl in IHs; invcs IHs; trivial.
+      - Case "NNRCimpBuildCollFor".
+        destruct p0; repeat destr sem.
+        specialize (IHs1 _ _ _ _ eqq).
+        specialize (IHs2 _ _ _ _ eqq0).
+        simpl in IHs1; invcs IHs1.
+        congruence.
+      - Case "NNRCimpPush".
+        invcs sem.
+        rewrite domain_update_first; trivial.
+      - Case "NNRCimpAssign".
+        invcs sem; trivial.
+      - Case  "NNRCimpFor".
+        destruct d; try discriminate.
+        clear eqq.
+        revert σ₁ ψ₁ σ₂ ψ₂ sem.
+        induction l; intros σ₁ ψ₁ σ₂ ψ₂ sem; invcs sem; trivial.
+        repeat destr H0.
+        specialize (IHl _ _ _ _ H0).
+        specialize (IHs _ _ _ _ eqq).
+        simpl in IHs; invcs IHs.
+        congruence.
+      - Case "NNRCimpIf".
+        destruct d; try discriminate.
+        destruct b; eauto.
+      - Case "NNRCimpEither".
+        destruct d; try discriminate;
+          repeat destr sem; invcs sem.
+        + specialize (IHs1 _ _ _ _ eqq0);
+            simpl in IHs1; invcs IHs1; trivial.
+        + specialize (IHs2 _ _ _ _ eqq0);
+            simpl in IHs2; invcs IHs2; trivial.
+    Qed.
+    
+  End props.
+  
+End NNRCimpEval.
+
+Notation "[ h , σc ; σ ⊢〚 e 〛 ]" := (nnrc_imp_expr_eval h σc σ e) : nnrc_imp. 
+Notation "[ h , σc ; σ , ψ ⊢〚 s 〛 ]" := (nnrc_imp_stmt_eval h σc σ ψ s) : nnrc_imp.
+
